# Soal 1

1. P(n) = 2 + 4 + 6 + ... + 2n = n(n+1)

   Basis Induksi
    ```
    n = 1
    P(1) = 2 = 1(1+1) = 2
    ```

   Langkah Indukasi 
    ```
    p(n+1) = n(n+1) + 2(n+1) = (n+1) (n+1+1)
	     n² + n + 2n + 2 = (n+1) (n+2)
	     n² + 3n + 2	 = n² + 2n + n + 2
					     = n² + 3n + 2
					     = n(n+1) + (2n + 2)
					     = n(n+1) + 2(n+1) 
    p(n+1)  = 2 + 4 + 6 + ...+ 2n + 2n + 2
    p(2)    = 2(1) + 2
    p(2)    = 4
    ```

# Soal 2

2. P(n) = 1 + 4 + 9 + ... + n² = 1/6n(n+1)(2n+1)

   Basis Induksi
    ```
    n = 1
    P(n) = 1 + 4 + 9 + ... + n² = 1/6n(n+1)(2n+1)
    P(1) = 1 + 4 + 9 + ... + 1² = 1/6(1)(1+1)(2(1)+1)
    P(1) = 1/6 * 6
    P(1) = 1 (benar)
    ```

   Langkah Induksi
    ```
    P(n)    = 1 + 4 + 9 + ... + n² = 1/6n(n+1)(2n+1)
    P(n+1)  = 1 + 4 + 9 + ... + n² + (n+1)² = 1/6n(n+1)(2n+1)
    P(n+1)  = P(n) + (n+1)²
            = 1/6 n(n+1)(2n+1) + (n+1)²
            = 1/6(n+1)[n(2n+1) + 6(n+1)]
            = n(2n+1) + 6(n+1)
            = 2n² + n + 6n + 6
            = 2n² + 7n + 6
            = (n+2)(2n+3)
            = 1/6(n+1)(n+2)(2n+3)
            = 1/6(n+1)((n+1)+1)(2(n+1)+1) (benar)


# Soal 3

3. P(n) = 2 + 6 + 12 + ... + n(n+1) = 1/3n(n+1)(n+2)

   Basis Induksi
    ```
    n = 1
    p(1) = 1 (1 + 1) = 2
    1/3(1)(1 + 1)(1 + 2) = 1/3(1)(2)(3) = 2
    ```

   Langkah Induksi
    ```
    P(k+1) = P(k)+(k+1)(k+2)
    P(k+1) = 3/1k(k+1)(k+2)+(k+1)(k+2)
    P(k+1) = (k+1)(k+2)(3/1k+1)
    P(k+1) = (k+1)(k+2)(k+3/3)
    P(k+1) = 1/3(k+1)(k+2)(k+3)
    ```