 1. P (n) = 2 + 4 + 6 + ... + 2n = n (n + 1)
	- P (1) = 2 (1) = 1 (1 + 1)
	2      =      2
	- P (n + 1) = 2 + 4 + 6 + ... + 2n + 2 (n + 1) = (n + 1) ((n + 1) + 1)
	n (n + 1) + (2n + 2) = (n + 1) (n + 2)
	n (n + 1) + (2n + 2) = n² + 2n + n + 2
	n (n + 1) + (2n + 2) = (n² + n) + (2n + 2)
	n (n + 1) + 2 (n + 1)  = n (n + 1) + 2 (n + 1)
	
2. P (n) = 1 + 4 + 9 + ... + n² = 1/6 n (n + 1) (2n + 1)
	- P (1) = (1)² = 1/6 (1) (1 + 1) (2 (1) + 1)
	1 = 1/6 (6)
	1 = 1
	- P (n + 1) = 1 + 4 + 9 + ... + n² + (n + 1)² = 1/6 (n + 1) ((n + 1) + 1) (2 (n + 1) + 1)
	1/6 (n + 1) (n + 2) (2n + 2 + 1)
	1/6 (n + 1) (n + 2) (2n + 3)
	1/6 (n + 1) (2n² + 3n + 4n + 6)
	1/6 (n + 1) (2n² + 7n + 6)
	1/6 (n + 1) (2n² + n) + (6n + 6)
	1/6 (n + 1) n (2n + 1) + 6 (n + 1)
	1/6 n (n + 1) (2n + 1) + 6 (n + 1)
	P (n) + 6 (n + 1)  = P (n + 1)
	1 + 4 + 9 + ... + n² + 6 (n + 1) = P (n + 1)

3. P (n) = 2 + 6 + 12 + ... + n (n + 1) = 1/3 n (n + 1) (n + 2)
	- P (1) = 1 (1 + 1) =  1/3 (1) (1 + 1) (1 + 2)
	2 = 1/3 (6)
	2 = 2
	- P (n + 1) = 2 + 6 + 12 + ... + n (n + 1) + (n + 1) ((n + 1) + 1 ) = 1/3 (n + 1) ((n + 1) + 1) ((n + 1) + 2)
	1/3 (n + 1) (n + 2) (n + 3)
	1/3 (n + 1) (n² + 3n + 2n + 6)
	1/3 (n + 1) (n² + 2n) + (3n + 6)
	1/3 (n + 1) n (n + 2) + 3 (n + 2)
	1/3 n (n + 1) (n + 2) + 3 (n + 2)
	P (n) + 3 (n + 2) = P (n + 1)
	2 + 6 + 12 + ... + n (n + 1) + 3 (n + 2) = P (n + 1)