# TUGAS POST TEST

  

1. p(n) = 2 + 4 + 6 + .... + 2n = n(n + 1)

Pemrosesannya :

p(n + 1) = n(n + 1) = (n + 1)((n + 1) + 1)

= (n + 1)(n + 2)

= (n^2 + n + 2n + 2)

= (n^2 + 3n + 2)

= (n^2 + n) + (2n + 2)

= n(n + 1) + 2(n + 1)

= p(n) + 2(n + 1)


Hasil : 

p(n + 1) = 2(n + 1) = 2 + 4 + 6 + ... + 2n + 2(n + 1)

TERBUKTI

---

  

2. p(n) = 1 + 4 + 9 + ... + n^2 = 1/6n (n + 1)(2n + 1)

Pemrosesannya  : 

p(n + 1) = 1/6 n(n + 1)(2n + 1) = 1/6 (n + 1)((n + 1) + 1)(2(n + 1) + 1)

= 1/6 (n + 1)(n + 2)((2n + 2) + 1)

= 1/6 (n + 1)(n + 2)(2n + 3)

= 1/6 (n + 1)(2n^2 + 4n + 3n + 6)

= 1/6 (n + 1)(2n^2 + 7n + 6)

= 1/6 (n + 1)(2n^2 + n) + (6n + 6)

= 1/6 (n + 1) n(2n + 1) + 6(n + 1)

= p(n) + 6(n + 1)

Hasil : 

p(n + 1) = 1 + 4 + 9 + ... + n^2 + 6(n + 1)

TERBUKTI

---

  

3. p(n) = 2 + 6 + 12 + ... + n(n + 1) = 1/3n (n + 1)(n + 2)

  

p(n + 1) = 1/3 n(n + 1)(n + 2) = 1/3 (n + 1)((n + 1) + 1)((n + 1) + 2)

Pemrosesannya

= 1/3 (n + 1)(n + 2)(n + 3)

= 1/3 (n + 1)(n^2 + 2n + 3n + 6)

= 1/3 (n + 1)(n^2 + 5n + 6)

= 1/3 (n + 1)(n^2 + 2n) + (3n + 6)

= 1/3 (n + 1) n(n + 2) + 3(n + 2)

= p(n) + 3(n + 2)

Hasil : 

p(n + 1) = 2 + 6 + 12 + ... + n(n + 1) + 3(n + 2)

TERBUKTI