## Soal 1
**Menguji Basis**
```
p(n) = 2 + 4 + 6 + ... + 2n = n (n+1)
 p(n) = n (n+1)
 p(1) = 1 (1+1)
 p(1) = 2
 ```

**Langkah Induksi**
```
p (n) = n (n+1)
p (n+1) = (n+1)(n+1)+1
p(n+1) = (n+1) (n+2)
p(n+1) = n^2 + 2n + 1 + n + 1
p(n+1) = n^2 + 3n + 2
p(n+1) = n (n+1) + 2n + 2
```

```
p(n+1) = 2 + 4 + 6 + .... + 2n + 2n + 2
misal n = 1
p(2)  = 2(1) + 2
p(2) = 4
```
**TERBUKTI**

## SOAL 2
**Menguji Basis**
```
p(n) = 1 + 4 + 9 + .... + n^2 = 1/6 n (n+1)(2n + 1)
p(n) = 1/6 n (n+1) (2n+1)
p(1) = 1/6 . 1 (1+1)(2.1 +1)
p(1) = 1/6 . 2 . 3
p(1) = 1
```
**Langkah Induksi**
```
p(n) = 1/6 n (n+1)(2n + 1)
p(n+1) = 1/6(n+1)(n+1+1)(2(n+1)+1)
       = 1/6 (n+1) (n+2)(2n+3)
       = 1/6 (n+1) (2n^2 + 3n + 4n + 6)
       = 1/6 (n+1) (2n^2 + 7n + 6)
       = 1/6 (n+1) (2n^2 + n + 6n + 6)
       = 1/6 (n+1) . n(2n + 1) + 6(n+1)
       = 1/6 n (n+1)(2n+1) + 6(n+1)
```

```
p(n+1) =  1 + 4 + 9 + .... + n^2 + 6(n+1)
misal n = 1
p(2) = 6 (1+1)
p(2) = 6 . 2
p(2) = 12

```
  **TERBUKTI**

## SOAL 3
**Menguji Basis**
```
p(n) = 2 + 6 + 12 + ... + n(n+1) = 1/3n(n+1)(n+2)
p(n) = 1/3n(n+1)(n+2)
p(1) = 1/3 . 1 (1+1)(1+2)
p(1) = 1/3 . 1 (2) (3)
p(1) = 1/3 . 6
p(1) = 2
```

**Langkah Induksi**
```
p(n) = 1/3n(n+1)(n+2)
p(n+1) = 1/3 (n+1) (n+1+1) (n+2+1)
p(n+1) = 1/3 (n+1) (n+2) (n+3)
p(n+1) = 1/3n(n+1)(n+2)+(n+1)(n+2)
```

```
p(n+1) = 2 + 6 + 12 + ... + n(n+1) + (n+1)(n+2)
misal p = 1
p(2) = (1+1)(1+2)
p(2) = (2)(3)
p(2) = 6
```
**TERBUKTI**


