### **Penyelesaian dengan Induksi Matematika**

#### **Pernyataan 1**  
\[
2 + 4 + 6 + \dots + 2n = n(n+1)
\]

- **Basis**:  
  \[
  2 = 1(1+1) \quad \text{Benar.}
  \]

- **Hipotesis**:  
  \[
  2 + 4 + \dots + 2k = k(k+1)
  \]

- **Induksi**:  
  \[
  2 + 4 + \dots + 2k + 2(k+1) = k(k+1) + 2(k+1) = (k+1)(k+2)
  \]

Pernyataan terbukti.

---

#### **Pernyataan 2**  
\[
1 + 4 + 9 + \dots + n^2 = \frac{1}{6}n(n+1)(2n+1)
\]

- **Basis**:  
  \[
  1 = \frac{1}{6}(1)(2)(3) \quad \text{Benar.}
  \]

- **Hipotesis**:  
  \[
  1 + 4 + \dots + k^2 = \frac{1}{6}k(k+1)(2k+1)
  \]

- **Induksi**:  
  \[
  1 + 4 + \dots + k^2 + (k+1)^2 = \frac{1}{6}k(k+1)(2k+1) + (k+1)^2
  \]
  \[
  = \frac{1}{6}(k+1)(k+2)(2k+1)
  \]

Pernyataan terbukti.

---

#### **Pernyataan 3**  
\[
2 + 6 + 12 + \dots + n(n+1) = \frac{1}{3}n(n+1)(n+2)
\]

- **Basis**:  
  \[
  2 = \frac{1}{3}(1)(2)(3) \quad \text{Benar.}
  \]

- **Hipotesis**:  
  \[
  2 + 6 + \dots + k(k+1) = \frac{1}{3}k(k+1)(k+2)
  \]

- **Induksi**:  
  \[
  2 + 6 + \dots + k(k+1) + (k+1)(k+2) = \frac{1}{3}k(k+1)(k+2) + (k+1)(k+2)
  \]
  \[
  = \frac{1}{3}(k+1)(k+2)(k+3)
  \]

Pernyataan terbukti.
